SP1Clean.lean
@@ -28,7 +28,7 @@ import SP1Clean.Chips.Memory.LoadWordChip
 import SP1Clean.Chips.Memory.LoadHalfChip
 import SP1Clean.Chips.Control.BranchChip.Aggregate
 import SP1Clean.Chips.Memory.LoadX0Chip
-import SP1Clean.Chips.ALU.ShiftRightChip.Aggregate
+import SP1Clean.Chips.ALU.ShiftRightChip.SailBridge
 import SP1Clean.Chips.ALU.DivRemChip.Circuit
 import SP1Clean.Chips.ALU.DivRemChip.SailBridge
 import SP1Clean.Reader.JTypeReader
@@ -38,7 +38,7 @@ import SP1Clean.Chips.Memory.StoreByteChip
 import SP1Clean.Chips.Control.JalChip.Circuit
 import SP1Clean.Chips.Control.JalChip.SailBridge
 import SP1Clean.Chips.ALU.MulChip.Aggregate
-import SP1Clean.Chips.ALU.ShiftLeftChip.Aggregate
+import SP1Clean.Chips.ALU.ShiftLeftChip.SailBridge
 import SP1Clean.Multiplicity
 import SP1Clean.Chips.Memory.MemoryGlobalChip
 import SP1Clean.Soundness
